Translation/Ty.lean
@@ -41,26 +41,20 @@ def Subst.Surface.Ty.translate (σ : Subst Surface.Ty) : Subst Core.Ty :=
 notation "⟦" σ "⟧" => Subst.Surface.Ty.translate σ
 
 
-inductive Surface.Translation.Ty (G : Surface.GlobalEnv) (G' : Core.GlobalEnv) :
-  Surface.KindEnv -> Surface.Ty -> Surface.Kind ->
-  Core.KindEnv -> Core.Ty -> Core.Kind -> Prop where
-| var {Δ : Surface.KindEnv} :
+inductive Surface.Translation.Ty (G : Surface.GlobalEnv) :
+  Surface.KindEnv -> Surface.Ty -> Surface.Kind -> Core.Ty -> Prop where
+| var :
   Δ[i]? = some K ->
-  Δ'[i]? = some K.translate ->
-  Translation.Ty G G' Δ t`#i K Δ' t#i K.translate
+  Translation.Ty G Δ t`#i K t#i
 | arrow :
-  Translation.Ty G G' Δ A `★ Δ' A' ★ ->
-  Translation.Ty G G' Δ B K Δ' B' K.translate ->
-  Translation.Ty G G' Δ (A `-:> B) `★ Δ' (A' -:> B') ★
-| «then» :
-  Translation.Ty G G' Δ A `◯ Δ' A' ◯ ->
-  Translation.Ty G G' Δ B K Δ' B' K.translate ->
-  Translation.Ty G G' Δ (A `=:> B) `★ Δ' (A' -:> B') ★
+  Translation.Ty G Δ A `★ A' ->
+  Translation.Ty G Δ B K B' ->
+  Translation.Ty G Δ (A `-:> B) `★ (A' -:> B')
 | app :
-  Translation.Ty G G' Δ A (.arrow K1 K2) Δ' A' (Surface.Kind.arrow K1 K2).translate ->
-  Translation.Ty G G' Δ B K1 Δ' B' K1.translate ->
-  Translation.Ty G G' Δ (A `• B) K2 Δ' (A' • B') K2.translate
+  Translation.Ty G Δ A (.arrow K1 K2) A' ->
+  Translation.Ty G Δ B K1 B' ->
+  Translation.Ty G Δ (A `• B) K2 (A' • B')
 | all :
-  Translation.Ty G G' Δ A K Δ' A' K.translate ->
-  Translation.Ty G G' (K::Δ) B `★ (K.translate::Δ') B' ★ ->
-  Translation.Ty G G' Δ (`∀[K]B) `★ Δ' (∀[K.translate] B') ★
+  Translation.Ty G Δ A K A' ->
+  Translation.Ty G (K::Δ) B `★ B' ->
+  Translation.Ty G Δ (`∀[K]B) `★ (∀[K.translate] B')
