Translation/Examples/Boolean.lean
@@ -19,7 +19,7 @@ not = λ x → case x of
                _ → False
 -/
 def Surface.notTerm : Surface.Term := λˢ[ .global "Bool" ]
-  matchˢ! `#0
+  matchˢ! 2 gt`#"Bool" `#0
          ([ g`#"True", g`#"False" ] : Vect 2 Term)
          ([ g`# "False", g`# "True" ])
          g`#"False"
@@ -34,17 +34,17 @@ def Surface.notTerm : Surface.Term := λˢ[ .global "Bool" ]
                        False → True
  -/
 def Surface.eqBool : Term := λˢ[ .global "Bool" ] λˢ[ .global "Bool" ]
-  matchˢ! `#1
+  matchˢ! 2 gt`#"Bool" `#1
    ([ g`#"True", g`#"False" ] : Vect 2 Term)
-   ([ matchˢ! `#0 ([ g`#"True", g`#"False" ] : Vect 2 Term) [ g`#"True", g`#"False"] g`#"False",
-      matchˢ! `#0 ([ g`#"True", g`#"False" ] : Vect 2 Term) [ g`# "False", g`# "False"] g`#"False"
+   ([ matchˢ! 2 gt`#"Bool" `#0 ([ g`#"True", g`#"False" ] : Vect 2 Term) [ g`#"True", g`#"False"] g`#"False",
+      matchˢ! 2 gt`#"Bool" `#0 ([ g`#"True", g`#"False" ] : Vect 2 Term) [ g`# "False", g`# "False"] g`#"False"
     ])
     g`#"False"
 
 
 -- #eval Surface.BoolCtx.infer
-#eval Surface.GlobalEnv.translate Surface.BoolCtx
+#eval! Surface.GlobalEnv.translate Surface.BoolCtx
 
-#eval do let gs' : Core.GlobalEnv <- Surface.BoolCtx.translate
-         let t' <- Surface.eqBool.translate gs' [] []
-         return t'
+#eval! do let gs' : Core.GlobalEnv <- Surface.BoolCtx.translate
+          let t' <- Surface.eqBool.translate gs' [] []
+          return t'
